made Address finite
Basically removed all `valid_node` related parts as a result.
Note that although in the future, the set of valid nodes may
change due to reconfiguration, the current definition of
`valid_node` will remain useless since in that case, we will have
to develop a `valid_node` which accepts time as an argument.

Systems/Address.v
@@ -1,53 +1,80 @@
-From Coq Require Import Lia List ssrbool.
+From Coq Require Import Lia List.
+From Coq Require ssrbool.
+Import (coercions) ssrbool.
 
 Module Type NetAddr.
 
-(* TODO validity and NoDup checks are everywhere. Consider changing the address type into a finite type eventually *)
-
-(* how about simply letting addr be a number within some range? any other things to notice here? *)
-(* TODO relate this with Byzantine assumption *)
-
-Parameter Address : Set. 
+Parameter Address : Set.
 Parameter Address_eqdec : forall (a1 a2 : Address), {a1 = a2} + {a1 <> a2}.
 
-Parameter is_byz : Address -> bool.
+(* restricting Address to be a finite type should be enough *)
 Parameter valid_nodes : list Address.
-
 Axiom valid_nodes_NoDup : NoDup valid_nodes.
+Axiom Address_is_finite : forall a : Address, In a valid_nodes.
 
 Definition N := length valid_nodes.
-Parameter t0 : nat.
+
+Parameter is_byz : Address -> bool.
 
 Definition num_byz := length (List.filter is_byz valid_nodes).
 
+(* t0: the threshold, indicating the maximum number of tolerable Byzantine nodes *)
+(* we do not assume the  *)
+Parameter t0 : nat.
+
 Axiom t0_lt_N : t0 < N.
 
-(* FIXME: trick *)
+(* FIXME: trick? instead of stating that valid_nodes is not empty, exploit the fact that 0 < N *)
 Definition Address_inhabitant : Address.
   destruct valid_nodes as [ | n ? ] eqn:E.
   2: exact n.
   assert (N = 0) as EN by (unfold N; now rewrite -> E).
   pose proof t0_lt_N.
-  lia.
+  rewrite EN in H.
+  now exfalso.
 Qed.
 
-(* TODO if we want properties about quorum, we need to quantify t0 here *)
-
-(* make valid_node explicitly decidable *)
-
+(*
 Definition valid_node n := In n valid_nodes.
 Definition is_valid_node n := In_dec Address_eqdec n valid_nodes.
 
 Axiom byz_is_valid : forall n, is_byz n -> valid_node n.
+*)
 
 (* this is not used. *)
+(*
 Axiom at_least_two_honest : exists n1 n2, 
   n1 <> n2 /\ 
   valid_node n1 /\
   valid_node n2 /\
   is_byz n1 = false /\ is_byz n2 = false.
-
-(* Parameter n : nat. *)
-(* Definition Address := 'I_n. *)
+*)
 
 End NetAddr.
+
+(* a simple example *)
+(* FIXME: seems like encountered a Coq bug? *)
+(*
+Module RealAddr <: NetAddr.
+
+From stdpp Require Import finite fin.
+
+Definition Address := fin 5.
+Definition Address_eqdec := @fin_dec 5.
+Definition valid_nodes := enum (fin 5).
+Lemma valid_nodes_NoDup : NoDup valid_nodes.
+Proof NoDup_enum (fin 5).
+Lemma Address_is_finite : forall a : Address, In a valid_nodes.
+Proof. setoid_rewrite <- elem_of_list_In. exact elem_of_enum. Qed.
+
+Definition is_byz : Address -> bool := fun _ => false.
+Definition t0 := 2.
+
+Definition N := length valid_nodes.
+Definition num_byz := length (List.filter is_byz valid_nodes).
+
+Fact t0_lt_N : t0 < N.
+Proof. unfold N, valid_nodes, t0. fold (card (fin 5)). rewrite fin_card. auto. Qed.
+
+End RealAddr.
+*)
